Progress on Blake2 unification

code/blake2/Hacl.Impl.Blake2.fst
@@ -541,9 +541,26 @@ let spec_update_block
     (init:nat)
     (d:Lib.ByteSequence.bytes{Seq.length d <= max_size_t
                              /\ init + Seq.length d <= max_size_t})
-    (i:nat{init + Seq.length d <= Spec.max_limb al /\ i < Seq.length d / v (size_block al)}) =
+    (i:nat{init + Seq.length d <= Spec.max_limb al /\ i < Seq.length d / v (size_block al)})
+    (hash:Spec.Blake2.hash_ws al)
+    =
     let block = Seq.sub #uint8 #(Seq.length d) d (i * v (size_block al)) (v (size_block al)) in
-    Spec.blake2_update_block al false (init + ((i + 1) * v (size_block al))) block
+    Spec.blake2_update_block al false (init + ((i + 1) * v (size_block al))) block hash
+
+
+val lemma_spec_eq_update_block:
+    (al:Spec.alg)
+    -> (init:nat)
+    -> (d:Lib.ByteSequence.bytes{Seq.length d <= max_size_t
+                             /\ init + Seq.length d <= max_size_t})
+    -> (i:nat{init + Seq.length d <= Spec.max_limb al /\ i < Seq.length d / v (size_block al)})
+    -> (hash:Spec.hash_ws al) ->
+    Lemma (
+      let f1 = spec_update_block al init d i hash in
+      let block = Seq.sub #uint8 #(Seq.length d) d (i * Spec.size_block al) (Spec.size_block al) in
+      let f2 = Spec.blake2_update_block al false (init + ((i + 1) * v (size_block al))) block hash in
+      f1 == f2)
+let lemma_spec_eq_update_block al init d i hash = ()
 
 
 val blake2_update_block_multi_single:
@@ -557,6 +574,9 @@ val blake2_update_block_multi_single:
     (requires (fun h -> live h hash /\ live h blocks /\ disjoint hash blocks))
     (ensures  (fun h0 _ h1 -> modifies1 hash h0 h1
                            /\ h1.[|hash|] == spec_update_block al (v prev) h0.[|blocks|] (v i) h0.[|hash|]))
+                           (* /\ ( *)
+                           (* let block = Seq.sub h0.[|blocks|] (v i * Spec.size_block al) (Spec.size_block al) in *)
+                           (* h1.[|hash|] == Spec.blake2_update_block al false (v prev + ((v i + 1) * Spec.size_block al)) block h0.[|hash|]) *)
 
 let blake2_update_block_multi_single al hash prev n i blocks =
   let curlen:size_t = (i +! 1ul) *! (size_block al) in
@@ -578,16 +598,18 @@ let spec_blake2_update_block_multi al prev n blocks s =
   repeati n (spec_update_block al prev blocks) s
 
 
-val lemma_eq_block_multi:
+val lemma_spec_eq_block_multi:
     al:Spec.alg
   -> prev:nat
   -> n:nat
-  -> blocks:Lib.ByteSequence.bytes{n * v (size_block al) == Seq.length blocks /\ prev + n * (Spec.size_block al) <= Spec.max_limb al}// /\ prev + Seq.length blocks <= max_size_t}
+  -> blocks:Lib.ByteSequence.bytes{n * Spec.size_block al == Seq.length blocks
+                                 /\ prev + n * (Spec.size_block al) <= Spec.max_limb al
+                                 /\ prev + Seq.length blocks <= max_size_t}
   -> hash:Spec.hash_ws al ->
-  Lemma (spec_blake2_update_block_multi al prev n blocks hash
-        == Spec.blake2_update_block_multi al prev n blocks hash)
+  Lemma (Spec.blake2_update_block_multi al prev n blocks hash
+        == spec_blake2_update_block_multi al prev n blocks hash)
 
-let lemma_eq_block_multi al prev n blocks hash =
+let lemma_spec_eq_block_multi al prev n blocks hash =
   let a = spec_blake2_update_block_multi al prev n blocks hash in
   let b = Spec.blake2_update_block_multi al prev n blocks hash in
   admit();
@@ -615,7 +637,7 @@ let blake2_update_block_multi al hash flag prev n blocks =
     Loops.unfold_repeati (v n) (spec h0) h0.[|hash|] (v i);
     blake2_update_block_multi_single al hash prev n i blocks);
   let h1 = ST.get() in
-  lemma_eq_block_multi al (v prev) (v n) h0.[|blocks|] h0.[|hash|]
+  lemma_spec_eq_block_multi al (v prev) (v n) h0.[|blocks|] h0.[|hash|]
 
 
 
